WIP adequacy

theories/examples/cmdc/cmdc_adequacy.v
@@ -1,126 +1,9 @@
 From iris.proofmode Require Import proofmode.
 From cap_machine Require Import logrel.
-From cap_machine Require Import cmdc_spec.
-(* From cap_machine Require Import compartment_layout. *)
-From stdpp Require Import base.
-From cap_machine Require Import switcher assert.
+From cap_machine Require Import compartment_layout.
+From cap_machine Require Import cmdc cmdc_spec.
+(* From cap_machine Require Import switcher assert. *)
 From cap_machine Require Import mkregion_helpers.
-
-Record cmpt : Type :=
-  mkCmpt {
-      cmpt_b_pcc : Addr;
-      cmpt_a_code : Addr;
-      cmpt_e_pcc : Addr;
-
-      cmpt_b_cgp : Addr;
-      cmpt_e_cgp : Addr;
-
-      cmpt_imports : list Word;
-      cmpt_code : list Word;
-      cmpt_data : list Word;
-
-      cmpt_import_size : (cmpt_b_pcc + length cmpt_imports)%a = Some cmpt_a_code;
-      cmpt_code_size : (cmpt_a_code + length cmpt_code)%a = Some cmpt_e_pcc;
-      cmpt_data_size : (cmpt_b_cgp + length cmpt_data)%a = Some cmpt_e_cgp;
-
-      code_data_disjoint :
-            (finz.seq_between cmpt_b_pcc cmpt_e_pcc)
-              ## (finz.seq_between cmpt_b_cgp cmpt_e_cgp)
-    }.
-
-Definition cmpt_pcc_region (C : cmpt) : list Addr :=
-  (finz.seq_between (cmpt_b_pcc C) (cmpt_e_pcc C)).
-
-Definition cmpt_cgp_region (C : cmpt) : list Addr :=
-  (finz.seq_between (cmpt_b_pcc C) (cmpt_e_pcc C)).
-
-Definition disjoint_cmpt (C1 C2 : cmpt) : Prop :=
-  let pcc1 := cmpt_pcc_region C1 in
-  let pcc2 := cmpt_pcc_region C2 in
-  let cgp1 := cmpt_cgp_region C1 in
-  let cgp2 := cmpt_cgp_region C2 in
-  pcc1 ## pcc2 ∧
-  pcc1 ## cgp2 ∧
-  cgp1 ## pcc2 ∧
-  cgp1 ## cgp2.
-
-Global Instance Cmpt_Disjoint : Disjoint cmpt := disjoint_cmpt.
-
-Definition cmpt_pcc_mregion (C: cmpt) : gmap Addr Word :=
-  mkregion (cmpt_b_pcc C) (cmpt_a_code C) (cmpt_imports C)
-  ∪ mkregion (cmpt_a_code C) (cmpt_e_pcc C) (cmpt_code C).
-
-Definition cmpt_cgp_mregion (C: cmpt) : gmap Addr Word :=
-  mkregion (cmpt_b_cgp C) (cmpt_e_cgp C) (cmpt_data C).
-
-(* Record cmptExportTbl : Type := *)
-(*   mkCmptExportTbl { *)
-(*       etlb_start : Addr ; *)
-(*       etlb_end : Addr ; *)
-(*     }. *)
-
-Record cmptSwitcher `{MachineParameters} : Type :=
-  mkCmptSwitcher {
-      b_switcher : Addr ;
-      e_switcher : Addr ;
-      a_switcher_cc : Addr ;
-      ot_switcher : OType ;
-
-      switcher_size :
-      (b_switcher + length switcher_instrs)%a = Some e_switcher ;
-
-      switcher_cc_entry_point :
-      (b_switcher + 1)%a = Some a_switcher_cc ;
-    }.
-
-Definition cmpt_switcher_region `{MachineParameters} (Cswitcher : cmptSwitcher) :=
-  (finz.seq_between (b_switcher Cswitcher) (e_switcher Cswitcher)).
-
-Definition cmpt_switcher_mregion `{MachineParameters} (Cswitcher : cmptSwitcher) : gmap Addr Word :=
-  let ot := (ot_switcher Cswitcher) in
-  let switcher_sealing := (WSealRange (true,true) Global ot (ot^+1)%ot ot) in
-  mkregion (b_switcher Cswitcher) (a_switcher_cc Cswitcher) [switcher_sealing]
-  ∪ mkregion (a_switcher_cc Cswitcher) (e_switcher Cswitcher) switcher_instrs.
-
-Definition switcher_disjoint
-  `{MachineParameters} (C : cmpt) (Cswitcher : cmptSwitcher) : Prop :=
-  let switcher := cmpt_switcher_code Cswitcher in
-  let pcc := cmpt_pcc_region C in
-  let cgp := cmpt_cgp_region C in
-  switcher ## pcc ∧ switcher ## cgp.
-
-Record cmptAssert `{MachineParameters} : Type :=
-  mkCmptAssert {
-      b_assert : Addr ;
-      e_assert : Addr ;
-      cap_assert : Addr ;
-      flag_assert : Addr ;
-
-      assert_code_size :
-      (b_assert + length (assert_subroutine_instrs cnull cnull cnull))%a = Some cap_assert ;
-      assert_cap_size :
-      (cap_assert + 1)%a = Some e_assert;
-
-      assert_flag_size :
-      (flag_assert + 1)%a = Some (flag_assert ^+ 1)%a;
-    }.
-
-Definition cmpt_assert_code `{MachineParameters} (Cassert : cmptAssert) :=
-  (finz.seq_between (b_assert Cassert) (e_assert Cassert)).
-
-Definition cmpt_assert_flag `{MachineParameters} (Cassert : cmptAssert) :=
-  (finz.seq_between (flag_assert Cassert) ((flag_assert Cassert) ^+1)%a).
-
-Definition assert_disjoint
-  `{MachineParameters} (C : cmpt) (Cassert : cmptAssert) : Prop :=
-  let assert_code := cmpt_assert_code Cassert in
-  let assert_flag := cmpt_assert_flag Cassert in
-  let pcc := cmpt_pcc_region C in
-  let cgp := cmpt_cgp_region C in
-  assert_code ## pcc ∧
-  assert_code ## cgp ∧
-  assert_flag ## pcc ∧
-  assert_flag ## cgp.
 
 Class memory_layout `{MachineParameters} := {
 
@@ -138,18 +21,196 @@ Class memory_layout `{MachineParameters} := {
     C_cmpt : cmpt ;
 
     (* disjointness *)
-    cmpts_disjoint :
+    cmpts_disjoints :
     main_cmpt ## B_cmpt
     ∧ main_cmpt ## C_cmpt
     ∧ B_cmpt ## C_cmpt ;
 
-    switcher_cmpt_disjoint :
-    switcher_disjoint main_cmpt switcher_cmpt
-    ∧ switcher_disjoint B_cmpt switcher_cmpt
-    ∧ switcher_disjoint C_cmpt switcher_cmpt ;
+    switcher_cmpt_disjoints :
+    switcher_cmpt_disjoint main_cmpt switcher_cmpt
+    ∧ switcher_cmpt_disjoint B_cmpt switcher_cmpt
+    ∧ switcher_cmpt_disjoint C_cmpt switcher_cmpt ;
 
-    assert_cmpt_disjoint :
-    assert_disjoint main_cmpt assert_cmpt
-    ∧ assert_disjoint B_cmpt assert_cmpt
-    ∧ assert_disjoint C_cmpt assert_cmpt ;
-}.
+    assert_cmpt_disjoints :
+    assert_cmpt_disjoint main_cmpt assert_cmpt
+    ∧ assert_cmpt_disjoint B_cmpt assert_cmpt
+    ∧ assert_cmpt_disjoint C_cmpt assert_cmpt ;
+
+    assert_switcher_disjoints :
+    assert_switcher_disjoint assert_cmpt switcher_cmpt;
+  }.
+
+Definition mk_initial_memory `{memory_layout} (mem: Mem) :=
+  mk_initial_switcher switcher_cmpt ∪
+    mk_initial_assert assert_cmpt ∪
+    mk_initial_cmpt main_cmpt ∪
+    mk_initial_cmpt B_cmpt ∪
+    mk_initial_cmpt C_cmpt.
+
+
+Definition is_initial_registers `{memory_layout} (reg: Reg) :=
+  reg !! PC = Some (WCap RX Global (cmpt_b_pcc main_cmpt) (cmpt_e_pcc main_cmpt) (cmpt_a_code main_cmpt)) ∧
+  reg !! cgp = Some (WCap RW Global (cmpt_b_cgp main_cmpt) (cmpt_e_cgp main_cmpt) (cmpt_b_cgp main_cmpt)) ∧
+  reg !! csp = Some (WCap RWL Local (b_switcher switcher_cmpt) (e_switcher switcher_cmpt) (b_switcher switcher_cmpt)) ∧
+  (∀ (r: RegName), r ∉ ({[ PC; cgp; csp ]} : gset RegName) → reg !! r = Some (WInt 0)).
+
+Definition is_initial_sregisters `{memory_layout} (sreg : SReg) :=
+  sreg !! MTDC = Some (WCap RWL Global
+                         (b_trusted_stack switcher_cmpt)
+                         (e_trusted_stack switcher_cmpt)
+                         (b_trusted_stack switcher_cmpt)).
+
+Definition is_initial_memory `{memory_layout} (mem: Mem) :=
+  let switcher_entry :=
+    WCap E_XSRW_ Global
+      (b_switcher switcher_cmpt)
+      (e_switcher switcher_cmpt)
+      (a_switcher_cc switcher_cmpt)
+  in
+  let B_f :=
+    SCap RO Global
+      (cmpt_exp_tbl_pcc B_cmpt)
+      (cmpt_exp_tbl_entries_end B_cmpt)
+      (cmpt_exp_tbl_entries_start B_cmpt)
+  in
+  let C_g :=
+    SCap RO Global
+      (cmpt_exp_tbl_pcc C_cmpt)
+      (cmpt_exp_tbl_entries_end C_cmpt)
+      (cmpt_exp_tbl_entries_start C_cmpt)
+  in
+
+  mem = mk_initial_memory mem
+  (* instantiating main *)
+  ∧ (cmpt_imports main_cmpt) =
+    cmdc_main_imports
+      (b_switcher switcher_cmpt) (e_switcher switcher_cmpt)
+      (a_switcher_cc switcher_cmpt) (ot_switcher switcher_cmpt)
+      (b_assert assert_cmpt) (e_assert assert_cmpt)
+      B_f C_g
+  ∧ (cmpt_code main_cmpt) = cmdc_main_code
+  ∧ (cmpt_data main_cmpt) = cmdc_main_data
+  ∧ (cmpt_exp_tbl_entries main_cmpt) = []
+
+  (* instantiating B *)
+  ∧ (cmpt_imports B_cmpt) = [] (* TODO imports !! *)
+  ∧ Forall is_z (cmpt_code B_cmpt) (* only instructions *)
+  ∧ Forall is_z (cmpt_data B_cmpt) (* TODO generalise: either z or in_region *)
+  ∧ (cmpt_exp_tbl_entries B_cmpt) = [WInt (switcher.encode_entry_point 1 0)]
+
+  (* instantiating C *)
+  ∧ (cmpt_imports C_cmpt) = [] (* TODO imports !! *)
+  ∧ Forall is_z (cmpt_code C_cmpt) (* only instructions *)
+  ∧ Forall is_z (cmpt_data C_cmpt) (* TODO generalise: either z or in_region *)
+  ∧ (cmpt_exp_tbl_entries C_cmpt) = [WInt (switcher.encode_entry_point 1 0)]
+.
+
+(* From iris.algebra Require Import auth agree excl gmap gset frac. *)
+(* From iris.proofmode Require Import proofmode. *)
+(* From cap_machine Require Import *)
+(*      stdpp_extra iris_extra *)
+(*      rules logrel fundamental. *)
+(* From cap_machine Require Import *)
+(*      stdpp_extra iris_extra *)
+(*      rules logrel fundamental region_invariants sts *)
+(*      region_invariants_revocation *)
+(*      region_invariants_allocation. *)
+(* From cap_machine.examples Require Import addr_reg_sample. *)
+(* From cap_machine.proofmode Require Export mkregion_helpers disjoint_regions_tactics. *)
+From iris.program_logic Require Import adequacy.
+From iris.base_logic Require Import invariants.
+Section Adequacy.
+  Context (Σ: gFunctors).
+  Context {inv_preg: invGpreS Σ}.
+  Context {mem_preg: gen_heapGpreS Addr Word Σ}.
+  Context {reg_preg: gen_heapGpreS RegName Word Σ}.
+  Context {sreg_preg: gen_heapGpreS SRegName Word Σ}.
+  Context {seal_store_preg: sealStorePreG Σ}.
+  Context {na_invg: na_invG Σ}.
+  Context {sts_preg: STS_preG Addr region_type Σ}.
+  Context {cname : CmptNameG}.
+  Context {heappreg: heapGpreS Σ}.
+  Context `{MP: MachineParameters}.
+  Context {B C: CmptName}.
+
+  Notation STS := (leibnizO (STS_states * STS_rels)).
+  Notation STS_STD := (leibnizO (STS_std_states Addr region_type)).
+  Notation CVIEW := (prodO STS_STD STS).
+  Notation WORLD := (gmapO CmptName CVIEW).
+
+   Definition flagN : namespace := nroot .@ "mcdc" .@ "assert_flag".
+
+  Lemma mcdc_adequacy' `{memory_layout}
+    (reg reg': Reg) (sreg sreg': SReg) (m m': Mem)
+    (es: list cap_lang.expr):
+    is_initial_registers reg →
+    is_initial_sregisters sreg →
+    is_initial_memory m →
+    rtc erased_step ([Seq (Instr Executable)], (reg, sreg, m)) (es, (reg', sreg', m')) →
+    m' !! (flag_assert assert_cmpt) = Some (WInt 0%Z).
+  Proof.
+    intros Hreg Hsreg Hm Hstep.
+    pose proof (@wp_invariance Σ cap_lang _ NotStuck) as WPI. cbn in WPI.
+    pose (fun (c: ExecConf) => c.2 !! (flag_assert assert_cmpt) = Some (WInt 0%Z)) as state_is_good.
+    specialize (WPI (Seq (Instr Executable)) (reg, sreg, m) es (reg', sreg', m')
+                  (state_is_good (reg', sreg', m'))).
+    eapply WPI. 2: assumption. intros Hinv κs. clear WPI.
+
+    destruct Hm as (Hm
+                    & main_imports & main_code & main_data & main_exp_tbl
+                    & B_imports & B_code & B_data & B_exp_tbl
+                    & C_imports & C_code & C_data & C_exp_tbl
+                   ).
+    iMod (gen_heap_init (reg:Reg)) as (reg_heapg) "(Hreg_ctx & Hreg & _)".
+    iMod (gen_heap_init (sreg:SReg)) as (sreg_heapg) "(Hsreg_ctx & Hsreg & _)".
+    iMod (gen_heap_init (m:Mem)) as (mem_heapg) "(Hmem_ctx & Hmem & _)".
+    iMod (seal_store_init) as (seal_storeg) "Hseal_store".
+
+    (* TODO something seems wrong, why do I allocate 2 STS ? *)
+    set W0 := (∅ : WORLD).
+    unshelve iMod (gen_sts_init B W0) as (stsg_B) "Hsts_B"; eauto. (*XX*)
+    unshelve iMod (gen_sts_init C W0) as (stsg_C) "Hsts_C"; eauto. (*XX*)
+    iMod (heap_init B) as (heapg_B) "HRELS_B".
+    iMod (heap_init C) as (heapg_C) "HRELS_C".
+    iMod (@na_alloc Σ na_invg) as (logrel_nais) "Hna".
+
+    pose ceriseg := CeriseG Σ Hinv mem_heapg reg_heapg sreg_heapg.
+    pose logrel_na_invs := Build_logrel_na_invs _ na_invg logrel_nais.
+    pose proof (
+        @cmdc_spec Σ ceriseg seal_storeg _ _ _ logrel_na_invs MP B C
+      ) as Spec.
+
+    (* pose proof cmpts_disjoints as Hcmpt_disjoint. *)
+    rewrite {2}Hm.
+    rewrite /mk_initial_memory.
+    iDestruct (big_sepM_union with "Hmem") as "[Hmem Hcmpt_C]".
+    { admit. }
+    iDestruct (big_sepM_union with "Hmem") as "[Hmem Hcmpt_B]".
+    { admit. }
+    iDestruct (big_sepM_union with "Hmem") as "[Hmem Hcmpt_main]".
+    { admit. }
+    iDestruct (big_sepM_union with "Hmem") as "[Hcmpt_switcher Hcmpt_assert]".
+    { admit. }
+
+    (* Assert *)
+    rewrite /mk_initial_assert.
+    iDestruct (big_sepM_union with "Hcmpt_assert") as "[Hassert Hassert_flag]".
+    { admit. }
+    rewrite /cmpt_assert_flag_mregion.
+    rewrite /mkregion.
+    rewrite finz_seq_between_singleton.
+    2: { admit. }
+    cbn.
+    iDestruct (big_sepM_insert with "Hassert_flag") as "[Hassert_flag _]"; first done.
+    iMod (inv_alloc flagN ⊤ (flag_assert assert_cmpt ↦ₐ WInt 0%Z) with "Hassert_flag")%I
+      as "#Hinv_assert_flag".
+    rewrite /cmpt_assert_code_mregion.
+
+
+    (* Switcher *)
+
+    iAssert (region W0 C) with "[HRELS_C]" as "Hr".
+    { rewrite region_eq /region_def. iExists ∅, ∅. iFrame.
+      rewrite /= !dom_empty_L //. repeat iSplit; eauto.
+      rewrite /region_map_def. by rewrite big_sepM_empty. }
+  Admitted.
