theories/examples/compartment_layout.v
@@ -1,146 +1,344 @@
 From cap_machine Require Import proofmode machine_parameters.
-From cap_machine Require Import switcher.
-
+From cap_machine Require Import switcher assert.
+From cap_machine Require Import disjoint_regions_tactics mkregion_helpers.
 
 Section CmptLayout.
   Context `{MP: MachineParameters}.
 
-  Record cmptSwitcher : Type :=
-    mkCmptSwitcher {
+  (* Class MemoryRegion := *)
+  (*   { *)
+  (*     A : Type ; *)
+  (*     region : A → list Addr *)
+  (*   }. *)
 
+  (* Global Instance MemoryRegion_Disjoint : Disjoint MemoryRegion. *)
+  (* Proof. *)
+  (*   rewrite /Disjoint. *)
+  (*   intros M1 M2; destruct M1,M2. *)
+  (*   exact (fun (m0 : A0) (m1 : A1)  (region0 m0) ## (region1 m1)). *)
+  (*   specialize (region0 A0). *)
+  (*   specialize (region1 m1). *)
+  (*   exact (region0 ## region1). *)
+  (* Defined. *)
+
+  Record cmpt : Type :=
+    mkCmpt {
+        cmpt_b_pcc : Addr;
+        cmpt_a_code : Addr;
+        cmpt_e_pcc : Addr;
+
+        cmpt_b_cgp : Addr;
+        cmpt_e_cgp : Addr;
+
+        cmpt_exp_tbl_pcc : Addr;
+        cmpt_exp_tbl_cgp : Addr;
+        cmpt_exp_tbl_entries_start : Addr;
+        cmpt_exp_tbl_entries_end : Addr;
+
+        cmpt_imports : list Word;
+        cmpt_code : list Word;
+        cmpt_data : list Word;
+        cmpt_exp_tbl_entries : list Word;
+
+        cmpt_import_size : (cmpt_b_pcc + length cmpt_imports)%a = Some cmpt_a_code;
+        cmpt_code_size : (cmpt_a_code + length cmpt_code)%a = Some cmpt_e_pcc;
+        cmpt_data_size : (cmpt_b_cgp + length cmpt_data)%a = Some cmpt_e_cgp;
+        cmpt_exp_tbl_pcc_size : (cmpt_exp_tbl_pcc + 1)%a = Some cmpt_exp_tbl_cgp;
+        cmpt_exp_tbl_cgp_size : (cmpt_exp_tbl_cgp + 1)%a = Some cmpt_exp_tbl_entries_start;
+        cmpt_exp_tbl_entries_size : (cmpt_exp_tbl_entries_end + length cmpt_exp_tbl_entries)%a = Some cmpt_exp_tbl_entries_end;
+
+        cmpt_disjointness :
+        ## [
+            (finz.seq_between cmpt_b_pcc cmpt_e_pcc) ;
+            (finz.seq_between cmpt_b_cgp cmpt_e_cgp) ;
+            (finz.seq_between cmpt_exp_tbl_pcc cmpt_exp_tbl_entries_end)
+          ]
+      }.
+
+  Definition cmpt_pcc_region (C : cmpt) : list Addr :=
+    (finz.seq_between (cmpt_b_pcc C) (cmpt_e_pcc C)).
+
+  Definition cmpt_cgp_region (C : cmpt) : list Addr :=
+    (finz.seq_between (cmpt_b_pcc C) (cmpt_e_pcc C)).
+
+  Definition cmpt_exp_tbl_region (C : cmpt) : list Addr :=
+    (finz.seq_between (cmpt_exp_tbl_pcc C) (cmpt_exp_tbl_entries_end C)).
+
+  Definition cmpt_region (C : cmpt) : list Addr :=
+   (cmpt_pcc_region C) ∪ (cmpt_cgp_region C) ∪ (cmpt_exp_tbl_region C).
+
+  Definition disjoint_cmpt (C1 C2 : cmpt) : Prop :=
+    cmpt_region C1 ## cmpt_region C2.
+
+  Global Instance Cmpt_Disjoint : Disjoint cmpt := disjoint_cmpt.
+
+  Definition cmpt_pcc_mregion (C: cmpt) : gmap Addr Word :=
+    mkregion (cmpt_b_pcc C) (cmpt_a_code C) (cmpt_imports C) ∪
+      mkregion (cmpt_a_code C) (cmpt_e_pcc C) (cmpt_code C).
+  Definition cmpt_cgp_mregion (C: cmpt) : gmap Addr Word :=
+    mkregion (cmpt_b_cgp C) (cmpt_e_cgp C) (cmpt_data C).
+  Definition cmpt_exp_tbl_mregion (C: cmpt) : gmap Addr Word :=
+    let pcc_word := WCap RX Global (cmpt_b_pcc C) (cmpt_e_pcc C) (cmpt_a_code C) in
+    let cgp_word := WCap RW Global (cmpt_b_cgp C) (cmpt_e_cgp C) (cmpt_b_cgp C) in
+    mkregion (cmpt_exp_tbl_pcc C) (cmpt_exp_tbl_cgp C) [pcc_word] ∪
+      mkregion (cmpt_exp_tbl_cgp C) (cmpt_exp_tbl_entries_start C) [cgp_word] ∪
+      mkregion (cmpt_exp_tbl_entries_start C) (cmpt_exp_tbl_entries_end C) (cmpt_exp_tbl_entries C)
+  .
+
+  Definition mk_initial_cmpt (C : cmpt) : gmap Addr Word :=
+    cmpt_pcc_mregion C ∪
+    cmpt_cgp_mregion C ∪
+    cmpt_exp_tbl_mregion C.
+
+  Record cmptSwitcher `{MachineParameters} : Type :=
+    mkCmptSwitcher {
         b_switcher : Addr ;
         e_switcher : Addr ;
         a_switcher_cc : Addr ;
         ot_switcher : OType ;
-        content_switcher : list Word;
-
-        content_switcher_correct :
-        content_switcher = (WSealRange (true,true) Global ot_switcher (ot_switcher^+1)%ot ot_switcher)::switcher_instrs;
 
         switcher_size :
-          (b_switcher + length content_switcher)%a = Some e_switcher ;
+        (b_switcher + length switcher_instrs)%a = Some e_switcher ;
 
         switcher_cc_entry_point :
-          (b_switcher + 1)%a = Some a_switcher_cc ;
+        (b_switcher + 1)%a = Some a_switcher_cc ;
 
+        b_trusted_stack : Addr;
+        e_trusted_stack : Addr;
+        trusted_stack_content : list Word;
+
+        trusted_stack_size :
+        (b_trusted_stack + length trusted_stack_content)%a = Some e_trusted_stack ;
+
+        (* compartment's stack *)
+        b_stack : Addr;
+        e_stack : Addr;
+        stack_content : list Word;
+
+        stack_size :
+        (b_stack + length stack_content)%a = Some e_stack ;
+
+        switcher_disjointness :
+        (finz.seq_between b_switcher e_switcher) ## (finz.seq_between b_trusted_stack e_trusted_stack)
+        ∧ (finz.seq_between b_switcher e_switcher) ## (finz.seq_between b_stack e_stack)
+        ∧ (finz.seq_between b_trusted_stack e_trusted_stack) ## (finz.seq_between b_stack e_stack)
       }.
 
-       codefrag b_assert (assert_subroutine_instrs rret rsrc1 rsrc2) ∗
-       ⌜(b_assert + length (assert_subroutine_instrs rret rsrc1 rsrc2))%a = Some cap_addr⌝ ∗
-       ⌜(cap_addr + 1)%a = Some e_assert⌝ ∗
+  Definition cmpt_switcher_code_region `{MachineParameters} (Cswitcher : cmptSwitcher) :=
+    (finz.seq_between (b_switcher Cswitcher) (e_switcher Cswitcher)).
 
+  Definition cmpt_switcher_trusted_stack_region `{MachineParameters} (Cswitcher : cmptSwitcher) :=
+    (finz.seq_between (b_trusted_stack Cswitcher) (e_trusted_stack Cswitcher)).
 
-  Record cmptAssert : Type :=
-    mkCmptSwitcher {
+  Definition cmpt_switcher_stack_region `{MachineParameters} (Cswitcher : cmptSwitcher) :=
+    (finz.seq_between (b_stack Cswitcher) (e_stack Cswitcher)).
 
+  Definition cmpt_switcher_region `{MachineParameters} (Cswitcher : cmptSwitcher) : list Addr :=
+    (cmpt_switcher_code_region Cswitcher)
+      ∪ (cmpt_switcher_trusted_stack_region Cswitcher)
+      ∪ (cmpt_switcher_stack_region Cswitcher).
+
+  Definition cmpt_switcher_code_mregion
+    `{MachineParameters} (Cswitcher : cmptSwitcher) : gmap Addr Word :=
+    let ot := (ot_switcher Cswitcher) in
+    let switcher_sealing := (WSealRange (true,true) Global ot (ot^+1)%ot ot) in
+    mkregion (b_switcher Cswitcher) (a_switcher_cc Cswitcher) [switcher_sealing]
+      ∪ mkregion (a_switcher_cc Cswitcher) (e_switcher Cswitcher) switcher_instrs .
+  Definition cmpt_switcher_trusted_stack_mregion
+    `{MachineParameters} (Cswitcher : cmptSwitcher) : gmap Addr Word :=
+    mkregion (b_trusted_stack Cswitcher) (e_trusted_stack Cswitcher) (trusted_stack_content Cswitcher).
+  Definition cmpt_switcher_stack_mregion
+    `{MachineParameters} (Cswitcher : cmptSwitcher) : gmap Addr Word :=
+    mkregion (b_stack Cswitcher) (e_stack Cswitcher) (stack_content Cswitcher).
+
+  Definition mk_initial_switcher `{MachineParameters} (Cswitcher : cmptSwitcher) : gmap Addr Word :=
+    cmpt_switcher_code_mregion Cswitcher ∪
+    cmpt_switcher_trusted_stack_mregion Cswitcher ∪
+    cmpt_switcher_stack_mregion Cswitcher.
+
+  Definition switcher_cmpt_disjoint
+    `{MachineParameters} (C : cmpt) (Cswitcher : cmptSwitcher) : Prop :=
+    (cmpt_switcher_region Cswitcher) ## (cmpt_region C).
+
+  Record cmptAssert `{MachineParameters} : Type :=
+    mkCmptAssert {
         b_assert : Addr ;
         e_assert : Addr ;
+        cap_assert : Addr ;
         flag_assert : Addr ;
-        content_assert : list Word;
-
-        content_assert_correct :
-        content_assert = assert_instrs++[WCap RW Global flag_assert (flag_assert ^+1)%a flag_assert];
 
         assert_code_size :
-        (assert_start + length content_assert)%a = Some assert_cap;
-        assert_size :
-          (b_assert + length content_assert)%a = Some e_assert ;
+        (b_assert + length assert_subroutine_instrs)%a = Some cap_assert ;
+        assert_cap_size :
+        (cap_assert + 1)%a = Some e_assert;
 
-        assert_cc_entry_point :
-          (b_assert + 1)%a = Some a_assert_cc ;
-
-
-        assert_size :
-          (b_assert + length assert_instrs)%a = Some e_assert ;
-
-        switcher_inbounds :
-        ( (b_switcher ^+ 1)%a <= a_switcher_cc < e_switcher)%a ;
-
-  (* (* assert library *) *)
-  (* assert_start : Addr; *)
-  (* assert_flag : Addr; *)
-  (* assert_end : Addr; *)
-
-  (* assert_code_size : *)
-  (*   (assert_start + length assert_subroutine_instrs)%a = Some assert_cap; *)
-  (* assert_cap_size : *)
-  (*   (assert_cap + 1)%a = Some assert_flag; *)
-  (* assert_flag_size : *)
-  (*   (assert_flag + 1)%a = Some assert_end; *)
-
-
-  (*       sealing_switcher_w : *)
-  (*       sealing_switcher = *)
-  (*       WSealRange (true,true) Global ot_switcher (ot_switcher^+1)%ot ot_switcher; *)
+        assert_flag_size :
+        (flag_assert + 1)%a = Some (flag_assert ^+ 1)%a;
       }.
 
+  Definition cmpt_assert_code_region `{MachineParameters} (Cassert : cmptAssert) :=
+    (finz.seq_between (b_assert Cassert) (e_assert Cassert)).
+  Definition cmpt_assert_flag_region `{MachineParameters} (Cassert : cmptAssert) :=
+    (finz.seq_between (flag_assert Cassert) ((flag_assert Cassert) ^+1)%a).
+  Definition cmpt_assert_region `{MachineParameters} (Cassert : cmptAssert) : list Addr :=
+    (cmpt_assert_code_region Cassert) ∪
+    (cmpt_assert_flag_region Cassert).
 
-  Definition is_switcher_cc (w : Word) : Prop :=
-    w = WCap E_XSR_ Global b_switcher e_switcher a_switcher_cc.
+  Definition cmpt_assert_code_mregion `{MachineParameters} (Cassert : cmptAssert) :=
+    mkregion (b_assert Cassert) (e_assert Cassert) assert_subroutine_instrs.
+  Definition cmpt_assert_flag_mregion `{MachineParameters} (Cassert : cmptAssert) :=
+    mkregion (flag_assert Cassert) ((flag_assert Cassert) ^+1)%a [WInt 0].
 
-  Definition is_valid_adv_import (w : Word) : Prop :=
-    is_sealed_with_o w ot_switcher \/ is_switcher_cc w.
+  Definition mk_initial_assert `{MachineParameters} (Cassert : cmptAssert) : gmap Addr Word :=
+    cmpt_assert_code_mregion Cassert ∪
+    cmpt_assert_flag_mregion Cassert.
 
-  (* TODO add the in_region condition *)
-  Definition is_valid_adv_data (b e : Addr) (w : Word)  : Prop :=
-    is_z w = true.
-  (* \/ in_region w b e. *)
+  Definition assert_cmpt_disjoint
+    `{MachineParameters} (C : cmpt) (Cassert : cmptAssert) : Prop :=
+    (cmpt_assert_region Cassert) ## (cmpt_region C).
 
-
-
-  Context { ot_switcher: OType } { b_switcher e_switcher a_switcher_cc : Addr }.
-
-Record cmpt : Type :=
-  mkCmpt {
-      cmpt_b_pcc : Addr;
-      cmpt_a_code : Addr;
-      cmpt_e_pcc : Addr;
-
-      cmpt_b_data : Addr;
-      cmpt_e_data : Addr;
-
-      cmpt_imports : list Word;
-      cmpt_code : list Word;
-      cmpt_data : list Word;
-
-      cmpt_import_size : (cmpt_b_pcc + length cmpt_imports)%a = Some cmpt_a_code;
-      cmpt_code_size : (cmpt_a_code + length cmpt_code)%a = Some cmpt_e_pcc;
-      cmpt_data_size : (cmpt_b_data + length cmpt_data)%a = Some cmpt_e_data;
-
-      code_data_disjoint :
-            (finz.seq_between cmpt_b_pcc cmpt_e_pcc)
-              ## (finz.seq_between cmpt_b_data cmpt_e_data)
-    }.
+  Definition assert_switcher_disjoint
+    `{MachineParameters} (Cassert : cmptAssert) (Cswitcher : cmptSwitcher) : Prop :=
+    (cmpt_assert_region Cassert) ## (cmpt_switcher_region Cswitcher).
 
 
-Record cmptAdv : Type :=
-  mkCmptAdv {
 
-      adv_cmpt : cmpt ;
+(*   Record cmptSwitcher : Type := *)
+(*     mkCmptSwitcher { *)
 
-      adv_cmpt_import_switcher_cc :
-        (cmpt_imports adv_cmpt) !! 0 = Some (WCap E_XSR_ Global b_switcher e_switcher a_switcher_cc);
-      adv_cmpt_importsWF :
-        Forall is_valid_adv_import (cmpt_imports adv_cmpt) ;
-      adv_cmpt_codeWF :
-        Forall is_z (cmpt_code adv_cmpt) ;
-      adv_cmpt_dataWF :
-        Forall (is_valid_adv_data (cmpt_b_data adv_cmpt) (cmpt_e_data adv_cmpt)) (cmpt_data adv_cmpt) ;
-    }.
+(*         b_switcher : Addr ; *)
+(*         e_switcher : Addr ; *)
+(*         a_switcher_cc : Addr ; *)
+(*         ot_switcher : OType ; *)
+(*         content_switcher : list Word; *)
+
+(*         content_switcher_correct : *)
+(*         content_switcher = (WSealRange (true,true) Global ot_switcher (ot_switcher^+1)%ot ot_switcher)::switcher_instrs; *)
+
+(*         switcher_size : *)
+(*           (b_switcher + length content_switcher)%a = Some e_switcher ; *)
+
+(*         switcher_cc_entry_point : *)
+(*           (b_switcher + 1)%a = Some a_switcher_cc ; *)
+
+(*       }. *)
+
+(*        codefrag b_assert (assert_subroutine_instrs rret rsrc1 rsrc2) ∗ *)
+(*        ⌜(b_assert + length (assert_subroutine_instrs rret rsrc1 rsrc2))%a = Some cap_addr⌝ ∗ *)
+(*        ⌜(cap_addr + 1)%a = Some e_assert⌝ ∗ *)
 
 
-Context { b_assert e_assert : Addr }.
-Record cmptMain : Type :=
-  mkCmptMain {
+(*   Record cmptAssert : Type := *)
+(*     mkCmptSwitcher { *)
 
-      main_cmpt : cmpt ;
+(*         b_assert : Addr ; *)
+(*         e_assert : Addr ; *)
+(*         flag_assert : Addr ; *)
+(*         content_assert : list Word; *)
 
-      main_cmpt_import_switcher_cc :
-        (cmpt_imports main_cmpt) !! 0 = Some (WCap E_XSR_ Global b_switcher e_switcher a_switcher_cc);
-      main_cmpt_assert :
-        (cmpt_imports main_cmpt) !! 1 = Some (WCap E_RX Global b_assert e_assert b_assert);
+(*         content_assert_correct : *)
+(*         content_assert = assert_instrs++[WCap RW Global flag_assert (flag_assert ^+1)%a flag_assert]; *)
 
-    }.
+(*         assert_code_size : *)
+(*         (assert_start + length content_assert)%a = Some assert_cap; *)
+(*         assert_size : *)
+(*           (b_assert + length content_assert)%a = Some e_assert ; *)
+
+(*         assert_cc_entry_point : *)
+(*           (b_assert + 1)%a = Some a_assert_cc ; *)
+
+
+(*         assert_size : *)
+(*           (b_assert + length assert_instrs)%a = Some e_assert ; *)
+
+(*         switcher_inbounds : *)
+(*         ( (b_switcher ^+ 1)%a <= a_switcher_cc < e_switcher)%a ; *)
+
+(*   (* (* assert library *) *) *)
+(*   (* assert_start : Addr; *) *)
+(*   (* assert_flag : Addr; *) *)
+(*   (* assert_end : Addr; *) *)
+
+(*   (* assert_code_size : *) *)
+(*   (*   (assert_start + length assert_subroutine_instrs)%a = Some assert_cap; *) *)
+(*   (* assert_cap_size : *) *)
+(*   (*   (assert_cap + 1)%a = Some assert_flag; *) *)
+(*   (* assert_flag_size : *) *)
+(*   (*   (assert_flag + 1)%a = Some assert_end; *) *)
+
+
+(*   (*       sealing_switcher_w : *) *)
+(*   (*       sealing_switcher = *) *)
+(*   (*       WSealRange (true,true) Global ot_switcher (ot_switcher^+1)%ot ot_switcher; *) *)
+(*       }. *)
+
+
+(*   Definition is_switcher_cc (w : Word) : Prop := *)
+(*     w = WCap E_XSR_ Global b_switcher e_switcher a_switcher_cc. *)
+
+(*   Definition is_valid_adv_import (w : Word) : Prop := *)
+(*     is_sealed_with_o w ot_switcher \/ is_switcher_cc w. *)
+
+(*   (* TODO add the in_region condition *) *)
+(*   Definition is_valid_adv_data (b e : Addr) (w : Word)  : Prop := *)
+(*     is_z w = true. *)
+(*   (* \/ in_region w b e. *) *)
+
+
+
+(*   Context { ot_switcher: OType } { b_switcher e_switcher a_switcher_cc : Addr }. *)
+
+(* Record cmpt : Type := *)
+(*   mkCmpt { *)
+(*       cmpt_b_pcc : Addr; *)
+(*       cmpt_a_code : Addr; *)
+(*       cmpt_e_pcc : Addr; *)
+
+(*       cmpt_b_data : Addr; *)
+(*       cmpt_e_data : Addr; *)
+
+(*       cmpt_imports : list Word; *)
+(*       cmpt_code : list Word; *)
+(*       cmpt_data : list Word; *)
+
+(*       cmpt_import_size : (cmpt_b_pcc + length cmpt_imports)%a = Some cmpt_a_code; *)
+(*       cmpt_code_size : (cmpt_a_code + length cmpt_code)%a = Some cmpt_e_pcc; *)
+(*       cmpt_data_size : (cmpt_b_data + length cmpt_data)%a = Some cmpt_e_data; *)
+
+(*       code_data_disjoint : *)
+(*             (finz.seq_between cmpt_b_pcc cmpt_e_pcc) *)
+(*               ## (finz.seq_between cmpt_b_data cmpt_e_data) *)
+(*     }. *)
+
+
+(* Record cmptAdv : Type := *)
+(*   mkCmptAdv { *)
+
+(*       adv_cmpt : cmpt ; *)
+
+(*       adv_cmpt_import_switcher_cc : *)
+(*         (cmpt_imports adv_cmpt) !! 0 = Some (WCap E_XSR_ Global b_switcher e_switcher a_switcher_cc); *)
+(*       adv_cmpt_importsWF : *)
+(*         Forall is_valid_adv_import (cmpt_imports adv_cmpt) ; *)
+(*       adv_cmpt_codeWF : *)
+(*         Forall is_z (cmpt_code adv_cmpt) ; *)
+(*       adv_cmpt_dataWF : *)
+(*         Forall (is_valid_adv_data (cmpt_b_data adv_cmpt) (cmpt_e_data adv_cmpt)) (cmpt_data adv_cmpt) ; *)
+(*     }. *)
+
+
+(* Context { b_assert e_assert : Addr }. *)
+(* Record cmptMain : Type := *)
+(*   mkCmptMain { *)
+
+(*       main_cmpt : cmpt ; *)
+
+(*       main_cmpt_import_switcher_cc : *)
+(*         (cmpt_imports main_cmpt) !! 0 = Some (WCap E_XSR_ Global b_switcher e_switcher a_switcher_cc); *)
+(*       main_cmpt_assert : *)
+(*         (cmpt_imports main_cmpt) !! 1 = Some (WCap E_RX Global b_assert e_assert b_assert); *)
+
+(*     }. *)
 
 
 
