theories/examples/cmdc/cmdc_spec.v
@@ -64,7 +64,7 @@ Section CMDC.
     (cgp_b ^+ 1)%a ∉ dom (std W_init C) ->
 
     (
-      na_inv logrel_nais Nassert (assert_inv ct3 ct0 ct1 b_assert e_assert a_flag)
+      na_inv logrel_nais Nassert (assert_inv b_assert e_assert a_flag)
       ∗ na_inv logrel_nais Nswitcher (switcher_inv b_switcher e_switcher a_cc_switcher ot_switcher)
       ∗ na_own logrel_nais E
 
@@ -411,10 +411,10 @@ Section CMDC.
 
     focus_block 4 "Hcode_main" as a_assert_c Ha_assert_c "Hcode" "Hcont"; iHide "Hcont" as hcont.
     iApply (assert_success_spec with
-             "[- $Hassert $Hna $HPC $Hct2 $Hct3 $Hct4 $Hct0 $Hct1
+             "[- $Hassert $Hna $HPC $Hct2 $Hct3 $Hct4 $Hct0 $Hct1 $Hcra
               $Hcode $Himport_assert]"); auto.
     { solve_addr. }
-    iNext; iIntros "(Hna & HPC & Hct2 & Hct3 & Hct4 & Hct0 & Hct1
+    iNext; iIntros "(Hna & HPC & Hct2 & Hct3 & Hct4 & Hcra & Hct0 & Hct1
                     & Hcode & Himport_assert)".
     subst hcont; unfocus_block "Hcode" "Hcont" as "Hcode_main".
 
@@ -682,10 +682,10 @@ Section CMDC.
 
     focus_block 9 "Hcode_main" as a_assert_b Ha_assert_b "Hcode" "Hcont"; iHide "Hcont" as hcont.
     iApply (assert_success_spec with
-             "[- $Hassert $Hna $HPC $Hct2 $Hct3 $Hct4 $Hct0 $Hct1
+             "[- $Hassert $Hna $HPC $Hct2 $Hct3 $Hct4 $Hcra $Hct0 $Hct1
               $Hcode $Himport_assert]"); auto.
     { solve_addr. }
-    iNext; iIntros "(Hna & HPC & Hct2 & Hct3 & Hct4 & Hct0 & Hct1
+    iNext; iIntros "(Hna & HPC & Hct2 & Hct3 & Hct4 & Hcra & Hct0 & Hct1
                     & Hcode & Himport_assert)".
     subst hcont; unfocus_block "Hcode" "Hcont" as "Hcode_main".
 
